Move lty infrastructure into correct place
- Content of dot_lty goes back into unary_lr;
- Move lty.v to a more sensible path.

theories/Dot/lr/unary_lr.v
@@ -1,1 +1,621 @@
-From D.Dot Require Export dot_lty.
+From iris.proofmode Require Import tactics.
+From D Require Export iris_prelude proper lty lr_syn_aux.
+From D Require Import pty_interp_subst_lemmas swap_later_impl.
+From D.Dot Require Import syn syn.path_repl.
+From D.Dot Require Export dlang_inst path_wp.
+From D.pure_program_logic Require Import lifting.
+
+Implicit Types (Σ : gFunctors).
+Implicit Types
+         (v w : vl) (e : tm) (d : dm) (ds : dms) (p : path)
+         (vs : vls) (ρ : var → vl) (l : label).
+
+Include LtyJudgements VlSorts dlang_inst.
+Include PTyInterpLemmas VlSorts dlang_inst.
+Export persistent_ty_interp_lemmas.
+
+(** The logical relation core is [V⟦T⟧], which interprets *open* types into
+    predicates over *closed* values. Hence, [V⟦T⟧ T args ρ v] uses its argument [ρ]
+    to interpret anything contained in T, but not things contained in v.
+
+    Semantic judgements must apply instead to open terms/value/paths; therefore,
+    they are defined using closing substitution on arguments of [interp].
+
+    Similar comments apply to [def_interp].
+
+    Additionally, both apply to *stamped* syntax, hence they only expect
+    [dtysem] and not [dtysyn] for type member definitions.
+ *)
+
+(** Override notations to specify scope. *)
+Notation "V⟦ T ⟧" := (pty_interpO T%ty).
+Notation "V⟦ Γ ⟧*" := (fmap (M := list) pty_interpO Γ).
+
+(* Use Program without its extended pattern-matching compiler; we only need
+   its handling of coercions. *)
+Unset Program Cases.
+
+Definition dlty Σ := env -> label -> iPPred dm Σ.
+Definition dltyO Σ := env -d> label -d> iPPredO dm Σ.
+Notation Dlty T := (λ ρ l, IPPred (λI d, T ρ l d)).
+
+Definition dslty Σ := env -> iPPred dms Σ.
+Definition dsltyO Σ := env -d> iPPredO dms Σ.
+Notation Dslty T := (λ ρ, IPPred (λI ds, T ρ ds)).
+
+Record ldlty Σ := LDlty {
+  ldlty_label : option label;
+  ldlty_car :> env -> iPPred dm Σ;
+}.
+Global Arguments LDlty {_} _%I _.
+Global Arguments ldlty_label {_} !_ /.
+Global Arguments ldlty_car {_} !_ /.
+
+Canonical Structure labelO := leibnizO label.
+
+Section ldlty_ofe.
+  Context {Σ}.
+  Let iso := (λ T : ldlty Σ, (ldlty_car T : _ -d> _, ldlty_label T)).
+  Instance ldlty_equiv : Equiv (ldlty Σ) := λ A B, iso A ≡ iso B.
+  Instance ldlty_dist : Dist (ldlty Σ) := λ n A B, iso A ≡{n}≡ iso B.
+  Lemma ldlty_ofe_mixin : OfeMixin (ldlty Σ).
+  Proof. exact: (iso_ofe_mixin iso). Qed.
+
+  Canonical Structure ldltyO := OfeT (ldlty Σ) ldlty_ofe_mixin.
+  Definition LDltyO ol (P : env -d> iPPredO dm Σ) : ldltyO := LDlty ol P.
+  Global Instance Proper_LDltyO: Proper ((≡) ==> (≡)) (LDltyO ol).
+  Proof. by solve_proper_prepare. Qed.
+End ldlty_ofe.
+Arguments ldltyO : clear implicits.
+Global Instance: Params (@LDltyO) 2 := {}.
+
+Record ldslty {Σ} := LDslty {
+  ldslty_car :> env -> iPPred dms Σ;
+  ldslty_olty : oltyO Σ 0;
+  ldslty_dlty : dlty Σ;
+  ldslty_commute {ds ρ} :
+    ldslty_car ρ (selfSubst ds) ⊢ ldslty_olty vnil ρ (vobj ds);
+  ldslty_mono {l d ds ρ} :
+    dms_hasnt ds l →
+    ldslty_car ρ ds ⊢ ldslty_car ρ ((l, d) :: ds);
+  ldslty_def2defs_head {l d ds ρ} :
+    ldslty_dlty ρ l d ⊢ ldslty_car ρ ((l, d) :: ds)
+}.
+
+Arguments ldslty : clear implicits.
+Arguments LDslty {_} _ _ _ _ _.
+Arguments ldslty_car {_} !_ /.
+Arguments ldslty_olty {_} !_ /.
+
+Section ldslty_ofe.
+  Context {Σ}.
+  Let iso := (λ T : ldslty Σ, (ldslty_car T : _ -d> _, ldslty_olty T)).
+  Instance ldslty_equiv : Equiv (ldslty Σ) := λ A B, iso A ≡ iso B.
+  Instance ldslty_dist : Dist (ldslty Σ) := λ n A B, iso A ≡{n}≡ iso B.
+  Lemma ldslty_ofe_mixin : OfeMixin (ldslty Σ).
+  Proof. exact: (iso_ofe_mixin iso). Qed.
+
+  (* Definition LDsltyO (P : env -d> iPPredO dm Σ) := LDslty P.
+  Global Instance : Proper ((≡) ==> (≡)) (LDltyO ol).
+  Proof. by solve_proper_prepare. Qed. *)
+End ldslty_ofe.
+Canonical Structure ldsltyO Σ := OfeT (ldslty Σ) ldslty_ofe_mixin.
+
+Section defs.
+  Context `{HdotG: dlangG Σ}.
+  Implicit Types (T : oltyO Σ 0) (TD : dlty Σ).
+  Definition mkDlty (φ : env -> label -> dm -> iProp Σ) `{∀ ρ l d, Persistent (φ ρ l d)} : dlty Σ :=
+    Dlty (λ ρ l, IPPred (φ ρ l)).
+  (* Definition mkLDlty optl (φ : envPred dm Σ) `{∀ ρ d, Persistent (φ ρ d)} : ldlty Σ :=
+    LDlty optl (λ ρ, IPPred (φ ρ)). *)
+
+  Definition lift_ldlty `{dlangG Σ} (φ : ldltyO Σ) : dltyO Σ := Dlty (λI ρ l d,
+    ⌜ ldlty_label φ = Some l ⌝ ∧ φ ρ d).
+  Global Arguments lift_ldlty /.
+
+  Definition dm_to_type d i (ψ : hoD Σ i) : iProp Σ :=
+    (∃ s σ, ⌜ d = dtysem σ s ⌝ ∧ s ↗n[ σ , i ] ψ)%I.
+End defs.
+
+(** Definitions for semantic (definition) typing *)
+Definition sdtp `{HdotG: dlangG Σ} l d Γ (φ : ldltyO Σ): iProp Σ :=
+  □∀ ρ, ⌜path_includes (pv (ids 0)) ρ [(l, d)] ⌝ → s⟦Γ⟧* ρ → lift_ldlty φ ρ l d.|[ρ].
+Global Arguments sdtp /.
+
+(** Multi-definition typing *)
+Definition sdstp `{HdotG: dlangG Σ} ds Γ (T : dsltyO Σ) : iProp Σ :=
+  ⌜wf_ds ds⌝ ∧ □∀ ρ, ⌜path_includes (pv (ids 0)) ρ ds ⌝ → s⟦Γ⟧* ρ → T ρ ds.|[ρ].
+Global Arguments sdstp /.
+
+(** Path typing *)
+Definition sptp `{HdotG: dlangG Σ} p i Γ (T : oltyO Σ 0): iProp Σ :=
+  □∀ ρ, s⟦Γ⟧* ρ -∗
+    ▷^i path_wp (p.|[ρ]) (λ v, oClose T ρ v).
+Global Arguments sptp /.
+
+(** Single-definition typing *)
+Notation "Γ s⊨ {  l := d  } : T" := (sdtp l d Γ T) (at level 64, d, l, T at next level).
+(** Multi-definition typing *)
+Notation "Γ s⊨ds ds : T" := (sdstp ds Γ T) (at level 74, ds, T at next level).
+Notation "Γ s⊨p p : τ , i" := (sptp p i Γ τ) (at level 74, p, τ, i at next level).
+Notation "d ↗n[ i  ] ψ" := (dm_to_type d i ψ) (at level 20).
+
+Section dm_to_type.
+  Context `{HdotG: dlangG Σ}.
+
+  Global Instance dm_to_type_persistent d i ψ: Persistent (d ↗n[ i ] ψ) := _.
+
+  Lemma dm_to_type_agree {d i ψ1 ψ2} args v : d ↗n[ i ] ψ1 -∗ d ↗n[ i ] ψ2 -∗ ▷ (ψ1 args v ≡ ψ2 args v).
+  Proof.
+    iDestruct 1 as (s σ ?) "#Hs1".
+    iDestruct 1 as (s' σ' ?) "#Hs2".
+    simplify_eq. by iApply (stamp_σ_to_type_agree args with "Hs1 Hs2").
+  Qed.
+
+  Lemma dm_to_type_intro d i s σ φ :
+    d = dtysem σ s → s ↝n[ i ] φ -∗ d ↗n[ i ] hoEnvD_inst σ φ.
+  Proof.
+    iIntros. iExists s, σ. iFrame "%".
+    by iApply stamp_σ_to_type_intro.
+  Qed.
+
+  Definition dm_to_type_eq d i ψ : dm_to_type d i ψ =
+    (∃ s σ, ⌜ d = dtysem σ s ⌝ ∧ s ↗n[ σ , i ] ψ)%I := eq_refl.
+
+  Global Opaque dm_to_type.
+End dm_to_type.
+
+Section SemTypes.
+  Context `{HdotG: dlangG Σ}.
+
+  Implicit Types (τ : oltyO Σ 0).
+   (* (ψ : vl -d> iPropO Σ) (φ : envD Σ)  *)
+
+  Program Definition lift_dinterp_vl (TD : ldltyO Σ) : oltyO Σ 0 :=
+    match ldlty_label TD with
+    | None => oBot
+    | Some l => olty0 (λI ρ v, ∃ d, ⌜v @ l ↘ d⌝ ∧ TD ρ d)
+    end.
+    (* check that the label in TD contains Some, else return false. *)
+  Global Instance Proper_lift_dinterp_vl : Proper ((≡) ==> (≡)) lift_dinterp_vl.
+  Proof.
+    rewrite /lift_dinterp_vl => ??[/=??]; repeat case_match;
+      simplify_eq; solve_proper_ho_equiv.
+  Qed.
+
+  (* Definition lift_dinterp_dms `{dlangG Σ} (T : dltyO Σ) : dsltyO Σ := Dslty (λI ρ ds,
+    ∃ l d, ⌜ dms_lookup l ds = Some d ⌝ ∧ T ρ l d).
+
+  Lemma sem_lift_dinterp_dms_vl_commute (T : ldltyO Σ) ds ρ l :
+    lift_dinterp_dms (lift_ldlty T) ρ (selfSubst ds) -∗
+    lift_dinterp_vl T vnil ρ (vobj ds).
+  Proof.
+    iDestruct 1 as (?l d ? ?) "H"; simplify_eq/=.
+    iExists d; iFrame. by iExists ds.
+  Qed. *)
+
+  Definition lift_dinterp_dms `{dlangG Σ} (TD : ldltyO Σ) : dsltyO Σ := Dslty (λI ρ ds,
+    ∃ l d, ⌜ dms_lookup l ds = Some d ⌝ ∧ lift_ldlty TD ρ l d).
+
+  Lemma sem_lift_dinterp_dms_vl_commute (T : ldltyO Σ) ds ρ :
+    lift_dinterp_dms T ρ (selfSubst ds) -∗
+    lift_dinterp_vl T vnil ρ (vobj ds).
+  Proof.
+    rewrite /lift_dinterp_vl.
+    iDestruct 1 as (l d ? ?) "H"; case_match; simplify_eq => //=.
+    iExists d; iFrame. iIntros "!%"; naive_solver.
+  Qed.
+
+  Lemma lift_dinterp_dms_mono T l ρ d ds
+    (Hl : dms_hasnt ds l):
+    lift_dinterp_dms T ρ ds -∗ lift_dinterp_dms T ρ ((l, d) :: ds).
+  Proof.
+    iDestruct 1 as (l' d' ??) "H".
+    iExists l', d'; iFrame. auto using dms_lookup_mono.
+  Qed.
+
+  Lemma sem_def2defs_head {T l ρ d ds}:
+    lift_ldlty T ρ l d -∗
+    lift_dinterp_dms T ρ ((l, d) :: ds).
+  Proof.
+    iDestruct 1 as (?) "H".
+    iExists l, d; iFrame. auto using dms_lookup_head.
+  Qed.
+
+  Program Definition LDsLift `{dlangG Σ} (T : ldltyO Σ) : ldsltyO Σ :=
+    LDslty (lift_dinterp_dms T) (lift_dinterp_vl T) (lift_ldlty T) _ _ _.
+  Next Obligation. intros. exact: sem_lift_dinterp_dms_vl_commute. Qed.
+  Next Obligation. intros. exact: lift_dinterp_dms_mono. Qed.
+  Next Obligation. intros. exact: sem_def2defs_head. Qed.
+
+  Program Definition LDsTop : ldslty Σ := LDslty (Dslty (λI _ _, True)) oTop (Dlty (λI ρ l d, True)) _ _ _.
+  Solve All Obligations with done.
+
+  Program Definition DBot : dlty Σ := Dlty (λI ρ l d, False).
+  Program Definition LDsBot : ldslty Σ := LDslty (Dslty (λI _ _, False)) oBot DBot _ _ _.
+  Solve All Obligations with done.
+
+  Program Definition LDsAnd (Tds1 Tds2 : ldslty Σ): ldslty Σ :=
+    LDslty (Dslty (λI ρ ds, Tds1 ρ ds ∧ Tds2 ρ ds)) (oAnd (ldslty_olty Tds1) (ldslty_olty Tds2)) DBot _ _ _.
+  Next Obligation. intros; iIntros "/= [??]". iSplit; by iApply ldslty_commute. Qed.
+  Next Obligation. intros; iIntros "/= [??]". iSplit; by iApply ldslty_mono. Qed.
+  Next Obligation. intros; iIntros "[]". Qed.
+
+  Definition mkLDlty ol (φ : env -> dm -> iProp Σ) `{∀ ρ d, Persistent (φ ρ d)} : ldlty Σ :=
+    LDlty ol (λ ρ, IPPred (φ ρ)).
+  Global Arguments mkLDlty /.
+
+  (* Rewrite using (higher) semantic kinds! *)
+  Definition oLDTMem l τ1 τ2 : ldltyO Σ := mkLDlty (Some l) (λI ρ d,
+    ∃ ψ, d ↗n[ 0 ] ψ ∧
+       □ ((∀ v, ▷ τ1 vnil ρ v → ▷ □ ψ vnil v) ∧
+          (∀ v, ▷ □ ψ vnil v → ▷ τ2 vnil ρ v))).
+  Global Instance Proper_oDTMem l : Proper ((≡) ==> (≡) ==> (≡)) (oLDTMem l).
+  Proof. rewrite /oLDTMem/= => ??? ???; f_equiv. solve_proper_ho_equiv. Qed.
+
+  Definition oTMem l τ1 τ2 := lift_dinterp_vl (oLDTMem l τ1 τ2).
+  Global Instance Proper_oTMem l : Proper ((≡) ==> (≡) ==> (≡)) (oTMem l).
+  Proof. rewrite /oTMem => ??? ???; f_equiv. solve_proper. Qed.
+
+  Definition oLDVMem l τ : ldltyO Σ := mkLDlty (Some l) (λI ρ d,
+    ∃ pmem, ⌜d = dpt pmem⌝ ∧ path_wp pmem (oClose τ ρ)).
+  Global Instance Proper_oLDVMem l : Proper ((≡) ==> (≡)) (oLDVMem l).
+  Proof. rewrite /oLDVMem/= => ???. f_equiv. solve_proper_ho_equiv. Qed.
+
+  Definition oVMem l τ := lift_dinterp_vl (oLDVMem l τ).
+  Global Instance Proper_oVMem l : Proper ((≡) ==> (≡)) (oVMem l).
+  Proof. rewrite /oVMem => ???; f_equiv. solve_proper. Qed.
+
+  Definition oSel {i} p l : oltyO Σ i :=
+    Olty (λI args ρ v, path_wp p.|[ρ]
+      (λ vp, ∃ ψ d, ⌜vp @ l ↘ d⌝ ∧ d ↗n[ i ] ψ ∧ ▷ □ ψ args v)).
+
+  Lemma oSel_pv {i} w l args ρ v :
+    oSel (pv w) l args ρ v ⊣⊢
+      ∃ ψ d, ⌜w.[ρ] @ l ↘ d⌝ ∧ d ↗n[ i ] ψ ∧ ▷ □ ψ args v.
+  Proof. by rewrite /= path_wp_pv. Qed.
+
+  Definition oSing `{dlangG Σ} p : olty Σ 0 := olty0 (λI ρ v, ⌜alias_paths p.|[ρ] (pv v)⌝).
+
+  (* Paolo: This definition is contractive (similarly to what's useful for
+     equi-recursive types).
+     However, I am not sure we need this; it'd be good to
+     write an example where this makes a difference.
+     I think that would be something like
+     nu x. { T = TNat; U = x.T -> x.T }:
+     mu (x: {T <: TNat; U <: x.T -> TNat}).
+     If the function type constructor is not contractive but only non-expansive,
+     typechecking this example needs to establish x.T <: TNat having in context
+     only x: {T <: TNat; U <: x.T -> TNat}.
+   *)
+  Definition oAll τ1 τ2 := olty0
+    (λI ρ v,
+    (∃ t, ⌜ v = vabs t ⌝ ∧
+     □ ∀ w, ▷ τ1 vnil ρ w → ▷ E⟦ τ2 ⟧ (w .: ρ) t.|[w/])).
+
+  Global Instance Proper_oAll : Proper ((≡) ==> (≡) ==> (≡)) oAll.
+  Proof. solve_proper_ho_equiv. Qed.
+
+  Definition oPrim b : olty Σ 0 := olty0 (λI ρ v, ⌜pure_interp_prim b v⌝).
+
+  (* Observe the naming pattern for semantic type constructors:
+  replace T by o. *)
+  Global Instance pinterp : PTyInterp ty Σ :=
+    fix pinterp (T : ty) : olty Σ 0 :=
+    let _ := pinterp : PTyInterp ty Σ in
+    match T with
+    | TTMem l L U => oTMem l V⟦ L ⟧ V⟦ U ⟧
+    | TVMem l T' => oVMem l V⟦ T' ⟧
+    | TAnd T1 T2 => oAnd V⟦ T1 ⟧ V⟦ T2 ⟧
+    | TOr T1 T2 => oOr V⟦ T1 ⟧ V⟦ T2 ⟧
+    | TLater T => oLater V⟦ T ⟧
+    | TPrim b => oPrim b
+    | TTop => oTop
+    | TBot => oBot
+    | TAll T1 T2 => oAll V⟦ T1 ⟧ V⟦ T2 ⟧
+    | TMu T => oMu V⟦ T ⟧
+    | TSel p l => oSel p l
+    | TSing p => oSing p
+    end.
+  Global Instance pinterp_lemmas: PTyInterpLemmas ty Σ.
+  Proof.
+    split => /=; induction T => args sb1 sb2 w /=;
+      properness; rewrite ?scons_up_swap ?hsubst_comp; trivial; by f_equiv => ?.
+  Qed.
+
+  Fixpoint ldef_interp (T : ty) : ldlty Σ :=
+    match T with
+    | TTMem l L U => oLDTMem l V⟦ L ⟧ V⟦ U ⟧
+    | TVMem l T' => oLDVMem l V⟦ T' ⟧
+    | _ => mkLDlty None (λI _ _, False)
+    end.
+  Notation "LD⟦ T ⟧" := (ldef_interp T).
+  Definition def_interp T l ρ d := lift_ldlty LD⟦ T ⟧ ρ l d.
+  Notation "D[ l ]⟦ T ⟧" := (def_interp T l).
+  Lemma ld_label_match T : ldlty_label LD⟦ T ⟧ = label_of_ty T.
+  Proof. by destruct T. Qed.
+
+  Program Definition defs_interp_and (interp1 interp2 : dslty Σ) : dslty Σ :=
+    Dslty (λI ρ ds, interp1 ρ ds ∧ interp2 ρ ds).
+
+  (* Reserved Notation "Ds⟦ T ⟧".
+  Fixpoint defs_interp T : dslty Σ :=
+    match T with
+    | TAnd T1 T2 => defs_interp_and Ds⟦T1⟧ Ds⟦T2⟧
+    | TTop => Dslty (λI ρ ds, True)
+    | _ => lift_dinterp_dms (LD⟦ T ⟧)
+    end
+  where "Ds⟦ T ⟧" := (defs_interp T). *)
+
+  Reserved Notation "Ds⟦ T ⟧".
+  Fixpoint ldefs_interp T : ldslty Σ :=
+    match T with
+    | TAnd T1 T2 => LDsAnd Ds⟦T1⟧ Ds⟦T2⟧
+    | TTop => LDsTop
+    | _ => LDsLift LD⟦ T ⟧
+    end
+  where "Ds⟦ T ⟧" := (ldefs_interp T).
+
+  Lemma def2defs_head {T l ρ d ds}:
+    lift_ldlty LD⟦ T ⟧ ρ l d -∗
+    Ds⟦ T ⟧ ρ ((l, d) :: ds).
+  Proof.
+    iIntros "#HT". iPoseProof "HT" as (Hl) "?".
+    destruct T; simplify_eq => //; by rewrite -ldslty_def2defs_head.
+  Qed.
+
+  Lemma lift_dsinterp_dms_vl_commute T ds ρ:
+    Ds⟦T⟧ ρ (selfSubst ds) -∗
+    V⟦T⟧ vnil ρ (vobj ds).
+  Proof.
+    rewrite ldslty_commute.
+    iInduction T as [] "IHT"; try iDestruct 1 as "[]"; [done | |iIntros "$"..].
+    iDestruct 1 as "/= [#H1 #H2]".
+    by iSplit; [> iApply "IHT"| iApply "IHT1"].
+  Qed.
+
+  Lemma defs_interp_mono T l ρ d ds:
+    dms_hasnt ds l →
+    Ds⟦T⟧ ρ ds -∗ Ds⟦T⟧ ρ ((l, d) :: ds).
+  Proof. apply ldslty_mono. Qed.
+
+  Definition idtp  Γ T l d     := sdtp l d  V⟦Γ⟧* LD⟦T⟧.
+  Definition idstp Γ T ds      := sdstp ds  V⟦Γ⟧* Ds⟦T⟧.
+  Definition ietp  Γ T e       := setp e    V⟦Γ⟧* V⟦T⟧.
+  Definition istpi Γ T1 T2 i j := sstpi i j V⟦Γ⟧* V⟦T1⟧ V⟦T2⟧.
+  Definition iptp  Γ T p i     := sptp p i  V⟦Γ⟧* V⟦T⟧.
+  (* Global Arguments idstp /. *)
+
+  (* Avoid auto-dropping box (and unfolding) when introducing judgments persistently. *)
+  Local Notation IntoPersistent' P := (IntoPersistent false P P).
+
+  Global Instance idtp_persistent Γ T l d: IntoPersistent' (idtp Γ T l d) | 0 := _.
+  Global Instance idstp_persistent Γ T ds: IntoPersistent' (idstp Γ T ds) | 0 := _.
+  Global Instance ietp_persistent Γ T e : IntoPersistent' (ietp Γ T e) | 0 := _.
+  Global Instance istpi_persistent Γ T1 T2 i j : IntoPersistent' (istpi Γ T1 T2 i j) | 0 := _.
+  Global Instance iptp_persistent Γ T p i : IntoPersistent' (iptp Γ T p i) | 0 := _.
+
+  Implicit Types (T : olty Σ 0) (Td : ldlty Σ) (Tds : dslty Σ).
+
+  Global Instance sdtp_persistent : IntoPersistent' (sdtp l d   Γ Td) | 0 := _.
+  Global Instance sdstp_persistent : IntoPersistent' (sdstp ds  Γ Tds) | 0 := _.
+  Global Instance setp_persistent : IntoPersistent' (setp e     Γ T) | 0 := _.
+  Global Instance sstpi_persistent : IntoPersistent' (sstpi i j Γ T1 T2) | 0 := _.
+  Global Instance sptp_persistent : IntoPersistent' (sptp p i   Γ T) | 0 := _.
+End SemTypes.
+
+Global Instance: Params (@oAll) 2 := {}.
+
+Section ldslty_defs.
+  Context `{dlangG Σ}.
+End ldslty_defs.
+
+Notation "LD⟦ T ⟧" := (ldef_interp T).
+Notation "D[ l ]⟦ T ⟧" := (def_interp T l).
+Notation "Ds⟦ T ⟧" := (ldefs_interp T).
+
+(* Backward compatibility. *)
+Notation "D*⟦ T ⟧" := (ldlty_car LD⟦ T ⟧).
+
+Notation "d ↗ ψ" := (dm_to_type 0 d ψ) (at level 20).
+Notation "G⟦ Γ ⟧" := s⟦ V⟦ Γ ⟧* ⟧*.
+
+(** Single-definition typing *)
+Notation "Γ ⊨ {  l := d  } : T" := (idtp Γ T l d) (at level 74, d, l, T at next level).
+(** Multi-definition typing *)
+Notation "Γ ⊨ds ds : T" := (idstp Γ T ds) (at level 74, ds, T at next level).
+(** Expression typing *)
+Notation "Γ ⊨ e : T" := (ietp Γ T e) (at level 74, e, T at next level).
+Notation "Γ ⊨p p : T , i" := (iptp Γ T p i) (at level 74, p, T, i at next level).
+Notation "Γ ⊨ T1 , i <: T2 , j " := (istpi Γ T1 T2 i j) (at level 74, T1, T2, i, j at next level).
+
+Import stamp_transfer.
+(** Judgment variants indexed by [gφ]. *)
+Notation "Γ ⊨[ gφ  ] { l := d  } : T" := (wellMappedφ gφ → idtp Γ T l d)%I (at level 74, d, l, T at next level).
+Notation "Γ ⊨ds[ gφ  ] ds : T" := (wellMappedφ gφ → idstp Γ T ds)%I (at level 74, ds, T at next level).
+Notation "Γ ⊨[ gφ  ] e : T" := (wellMappedφ gφ → ietp Γ T e)%I (at level 74, e, T at next level).
+Notation "Γ ⊨p[ gφ  ] p : T , i" := (wellMappedφ gφ → iptp Γ T p i)%I (at level 74, p, T, i at next level).
+Notation "Γ ⊨[ gφ  ] T1 , i <: T2 , j" := (wellMappedφ gφ → istpi Γ T1 T2 i j)%I (at level 74, T1, T2, i, j at next level).
+
+Section SampleTypingLemmas.
+  Context `{HdotG: dlangG Σ}.
+  Implicit Types (τ L T U : olty Σ 0).
+
+  Lemma def_interp_tvmem_eq l T p ρ :
+    lift_ldlty (oLDVMem l T) ρ l (dpt p) ⊣⊢
+    path_wp p (oClose T ρ).
+  Proof.
+    rewrite /lift_ldlty/=; iSplit. by iDestruct 1 as (_ pmem [= ->]) "$".
+    iIntros "H"; iSplit; first done; iExists p. by auto.
+  Qed.
+
+  Context {Γ : sCtx Σ}.
+
+  Lemma sSub_Refl T i : Γ s⊨ T, i <: T, i.
+  Proof. by iIntros "!> **". Qed.
+
+  Lemma sSub_Trans {T1 T2 T3 i1 i2 i3} : Γ s⊨ T1, i1 <: T2, i2 -∗
+                                      Γ s⊨ T2, i2 <: T3, i3 -∗
+                                      Γ s⊨ T1, i1 <: T3, i3.
+  Proof.
+    iIntros "#Hsub1 #Hsub2 !> * #Hg #HT".
+    iApply ("Hsub2" with "[//] (Hsub1 [//] [//])").
+  Qed.
+
+  Lemma sSub_Eq T U i j :
+    Γ s⊨ T, i <: U, j ⊣⊢
+    Γ s⊨ iterate oLater i T, 0 <: iterate oLater j U, 0.
+  Proof. cbn. by setoid_rewrite iterate_oLater_later. Qed.
+
+  Lemma pty_interp_subst (T : ty) σ : V⟦ T.|[σ] ⟧ ≡ V⟦ T ⟧.|[σ].
+  Proof. intros ???; apply interp_subst_compose_ind. Qed.
+
+  (* Lemma swap0 T σ args ρ v : V⟦ T.|[σ] ⟧ args ρ v ≡ (V⟦ T ⟧).|[σ] args ρ v.
+  Proof. apply interp_subst_compose_ind. Qed. *)
+
+  Lemma lift_olty_eq {i} {τ1 τ2 : oltyO Σ i} {args ρ v} :
+    τ1 ≡ τ2 → τ1 args ρ v ≡ τ2 args ρ v.
+  Proof. apply. Qed.
+End SampleTypingLemmas.
+
+(** * Proper instances. *)
+Section Propers.
+  (** This instance doesn't allow setoid rewriting in the function argument
+  to [iterate]. That's appropriate for this project. *)
+  Global Instance: Params (@iterate) 3 := {}.
+  Global Instance Proper_iterate {n} {A : ofeT} (f : A -> A) :
+    Proper (equiv ==> equiv) f →
+    Proper (equiv ==> equiv) (iterate f n).
+  Proof.
+    elim: n => [|n IHn] Hp x y Heq; rewrite ?(iterate_0, iterate_S) //.
+    f_equiv. exact: IHn.
+  Qed.
+
+  Context `{HdotG: dlangG Σ}.
+
+  Global Instance Proper_lift_ldlty : Proper ((≡) ==> (≡)) (lift_ldlty (Σ := Σ)).
+  Proof. move => [l1 P1] [l2 P2] [/= Heq]. solve_proper_ho_equiv. Qed.
+  Global Instance: Params (@lift_ldlty) 5 := {}.
+
+  Global Instance Proper_env_oltyped : Proper ((≡) ==> (=) ==> (≡)) env_oltyped.
+  Proof.
+    move => + + /equiv_Forall2 + + _ <-.
+    elim => [|T1 G1 IHG1] [|T2 G2] /=; [done|inversion 1..|] =>
+      /(Forall2_cons_inv _ _ _ _) [HT HG] ρ; f_equiv; [apply IHG1, HG|apply HT].
+  Qed.
+  Global Instance: Params (@env_oltyped) 2 := {}.
+
+  (** ** Judgments *)
+  Global Instance Proper_sstpi i j : Proper ((≡) ==> (≡) ==> (≡) ==> (≡)) (sstpi i j).
+  Proof.
+    solve_proper_ho_equiv.
+    (* intros ?? HG ?? H1 ?? H2; simplify_eq/=.
+    properness; [by rewrite HG|apply H1|apply H2]. *)
+  Qed.
+  Global Instance Proper_sstpi_flip i j :
+    Proper ((≡) --> (≡) --> (≡) --> flip (≡)) (sstpi i j).
+  Proof. apply: flip_proper_4. Qed.
+  Global Instance: Params (@sstpi) 4 := {}.
+
+
+  Global Instance Proper_setp e : Proper ((≡) ==> (≡) ==> (≡)) (setp e).
+  Proof.
+    solve_proper_ho_equiv.
+    (* intros ?? HG ?? HT ???; simplify_eq/=. by properness; [rewrite HG|apply HT]. *)
+  Qed.
+  Global Instance Proper_setp_flip e :
+    Proper (flip (≡) ==> flip (≡) ==> flip (≡)) (setp e).
+  Proof. apply: flip_proper_3. Qed.
+  Global Instance: Params (@setp) 3 := {}.
+
+  Global Instance Proper_sdtp l d : Proper ((≡) ==> (≡) ==> (≡)) (sdtp l d).
+  Proof.
+    move => ??? [??] [??] [??]; simplify_eq/=; properness => //;
+      solve_proper_ho_equiv.
+  Qed.
+  Global Instance Proper_sdtp_flip l d : Proper (flip (≡) ==> flip (≡) ==> flip (≡)) (sdtp l d).
+  Proof. apply: flip_proper_3. Qed.
+  Global Instance: Params (@sdtp) 4 := {}.
+End Propers.
+
+Section defs.
+  Context `{HdotG: dlangG Σ}.
+
+  (* We don't expose the binding lemmas on this wrapper, only on the
+     underlying interface. *)
+  (* Global Instance interp_lemmas: TyInterpLemmas ty Σ.
+  Proof. split => /= *; apply persistent_ty_interp_lemmas.interp_subst_compose_ind. Qed. *)
+
+  Lemma def_interp_tvmem_eq' l (T : ty) p ρ:
+    D[ l ]⟦ TVMem l T ⟧ ρ (dpt p) ⊣⊢
+    path_wp p (V⟦ T ⟧ vnil ρ).
+  Proof. apply def_interp_tvmem_eq. Qed.
+
+  Lemma iterate_TLater_oLater i T:
+    V⟦iterate TLater i T⟧ ≡ iterate oLater i V⟦T⟧.
+  Proof. elim: i => [//|i IHi] ???. by rewrite !iterate_S /= (IHi _ _ _). Qed.
+
+  Lemma iterate_TLater_later T n args ρ v:
+    V⟦ iterate TLater n T ⟧ args ρ v ≡ (▷^n V⟦ T ⟧ args ρ v)%I.
+  Proof.
+    by rewrite (iterate_TLater_oLater n T _ _ _) iterate_oLater_later.
+  Qed.
+
+  Context {Γ : ctx}.
+
+  Lemma Sub_Refl T i : Γ ⊨ T, i <: T, i.
+  Proof. apply sSub_Refl. Qed.
+
+  Lemma Sub_Trans {T1 T2 T3 i1 i2 i3} :
+    Γ ⊨ T1, i1 <: T2, i2 -∗ Γ ⊨ T2, i2 <: T3, i3 -∗
+    Γ ⊨ T1, i1 <: T3, i3.
+  Proof. apply sSub_Trans. Qed.
+
+  Lemma Sub_Eq T U i j :
+    Γ ⊨ T, i <: U, j ⊣⊢
+    Γ ⊨ iterate TLater i T, 0 <: iterate TLater j U, 0.
+  Proof. by rewrite /istpi sSub_Eq !iterate_TLater_oLater. Qed.
+
+  Lemma T_Var x τ
+    (Hlook : Γ !! x = Some τ):
+    (*──────────────────────*)
+    Γ ⊨ of_val (ids x) : shiftN x τ.
+  Proof.
+    rewrite /ietp (pty_interp_subst τ (ren (+x))). apply sT_Var.
+    by rewrite list_lookup_fmap Hlook.
+  Qed.
+End defs.
+
+Import dlang_adequacy adequacy.
+Theorem s_adequacy_dot_sem Σ `{HdlangG: dlangPreG Σ} `{SwapPropI Σ} {e Ψ}
+  (τ : ∀ `{dlangG Σ}, olty Σ 0)
+  (Himpl : ∀ (Hdlang: dlangG Σ) v, oClose τ ids v -∗ ⌜Ψ v⌝)
+  (Hlog : ∀ `{dlangG Σ} `(!SwapPropI Σ), allGs ∅ ==∗ [] s⊨ e : τ):
+  ∀ σ, adequate NotStuck e σ (λ v _, Ψ v).
+Proof.
+  eapply (adequacy_dlang _); [apply Himpl | iIntros (??) "Hgs"].
+  iMod (Hlog with "Hgs") as "#Htyp".
+  iEval rewrite -(hsubst_id e). iApply ("Htyp" $! ids with "[//]").
+Qed.
+
+Theorem adequacy_dot_sem Σ `{HdlangG: dlangPreG Σ} `{SwapPropI Σ} {e Ψ T}
+  (Himpl : ∀ (Hdlang: dlangG Σ) v, V⟦ T ⟧ vnil ids v -∗ ⌜Ψ v⌝)
+  (Hlog : ∀ `{dlangG Σ} `(!SwapPropI Σ), allGs ∅ ==∗ [] ⊨ e : T):
+  ∀ σ, adequate NotStuck e σ (λ v _, Ψ v).
+Proof. exact: (s_adequacy_dot_sem Σ (λ _, V⟦T⟧)). Qed.
+
+Corollary s_safety_dot_sem Σ `{HdlangG: dlangPreG Σ} `{SwapPropI Σ} {e}
+  (τ : ∀ `{dlangG Σ}, olty Σ 0)
+  (Hwp : ∀ `{dlangG Σ} `(!SwapPropI Σ), allGs ∅ ==∗ [] s⊨ e : τ):
+  safe e.
+Proof. apply adequate_safe, (s_adequacy_dot_sem Σ τ), Hwp; naive_solver. Qed.
+
+Corollary safety_dot_sem Σ `{HdlangG: dlangPreG Σ} `{SwapPropI Σ} {e T}
+  (Hwp : ∀ `{dlangG Σ} `(!SwapPropI Σ), allGs ∅ ==∗ [] ⊨ e : T):
+  safe e.
+Proof. exact: (s_safety_dot_sem Σ (λ _, V⟦T⟧)). Qed.
+
+(** Backward compatibility. *)
+Definition ty_interp `{!dlangG Σ} T : envD Σ := pty_interpO T vnil.
+Notation "⟦ T ⟧" := (ty_interp T).
+Arguments ty_interp {_ _} _ /.
